ulib/FStar.All.fst
@@ -19,7 +19,7 @@ include FStar.ST
 include FStar.Exn
 
 let all_pre = all_pre_h heap
-let all_post' (a : Type) (pre:Type) = all_post_h' heap a pre
+let all_post' (a : Type) (pre:prop) = all_post_h' heap a pre
 let all_post (a : Type) = all_post_h heap a
 let all_wp (a : Type) = all_wp_h heap a
 new_effect ALL  = ALL_h heap
